In this appendix we show how the sums in equations \eqref{z2i:eq:appendixable1} and 
\eqref{z2i:eq:appendixable2} are calculated.

\subsection{Auxiliary results}

For ease of reading let us repeat from \ref{sec:z2i} that 
$i\in \set{1,2,\ldots,m}$ and the definition of $\xi_i$ is as follows:

\begin{equation}
	\xi_i = \frac{1-(-2)^{i+1}} 3.
\end{equation}

Evaluate the following expressions:

\begin{equation}
	\label{appendix:eq:xi1}
	\xi_i^2
	 = \frac 1 9 \left(
		1 + (-2)^{i+2} + 2^{2i+2}
	 \right);
\end{equation}

\begin{equation}
	\label{appendix:eq:xi2}
	\xi_i (\xi_i - 2 \xi_s)
	 = -\frac 1 9 \left(
		1 + (-2)^{s+2} - 2^{2i+2} - (-2)^{s+i+3}
	 \right);
\end{equation}

\begin{equation}
	\label{appendix:eq:xi3}
	\xi_{r+1} (\xi_{r+1} + 2(-2)^r)
	= \frac 1 9 \left(
		1 + (-2)^{r+1} + (-2)^{2r+3}
	\right)
\end{equation}

We will also need the values of the following sums:

\begin{equation}
	\label{appendix:eq:sum1}
	\sum\limits_{i<s} 2^{-i} = 1 - 2^{1-s};
\end{equation}

\begin{equation}
	\label{appendix:eq:sum2}
	\sum\limits_{i<s}  2^{-i} (-2)^{s+2}
	= (-1)^s (2^{s+2} - 2^3);
\end{equation}

\begin{equation}
	\label{appendix:eq:sum3}
	\sum\limits_{i<s} 2^{-i} 2^{2i+2}
	= \sum\limits_{i<s} 2^{i+2}
	= 2^{s+2} - 2^3;
\end{equation}

\begin{equation}
	\label{appendix:eq:sum4}
	\sum\limits_{i<s} 2^{-i} (-2)^{s+i+3}
	= 2^{s+3} (-1)^{s+1} \sum\limits_{i<s} (-1)^i
	= 2^{s+2} (1+(-1)^s);
\end{equation}

\begin{equation}
	\label{appendix:eq:sum5}
	\sum\limits_{i \leq r} 2^{-i} = 1 - 2^{-r};
\end{equation}

\begin{equation}
	\label{appendix:eq:sum6}
	\sum\limits_{i \leq r} 2^{-i} (-2)^{i+2}
	= -2 (1 - (-1)^r);
\end{equation}

\begin{equation}
	\label{appendix:eq:sum7}
	\sum\limits_{i \leq r} 2^{-i} 2^{2i+2}
	= 2^3 (2^r - 1).
\end{equation}

\subsection{Evaluation of expression in \eqref{z2i:eq:appendixable1}}

Let us start by separating case of $i=s$ out of the sum, factoring out
$2^m$ and grouping the terms. We can evaluate the obtained
expression using the notes on $\xi_i$ from the previous section:

\begin{equation}
	\begin{split}
		& \sum\limits_{i<s} 2^{m-i} \xi_i^2 - 2 \xi_s \sum\limits_{i \leq s}  2^{m-i} \xi_i \\
		= & 2^m \left[
			-2^{1-s} \xi_s^2 
			+ \sum\limits_{i<s} 2^{-i} \xi_i (\xi_i - 2\xi_s)
		\right] \\
		= & - \frac{2^m}9 \left[
			2^{1-s} (1-(-2)^{s+1})^2
			+ \sum\limits_{i<s} 2^{-i} \left(
				1 + (-2)^{s+2} - 2^{2i+2} - (-2)^{s+i+3}
			\right)
		\right].
	\end{split}
\end{equation}

The sum can be expanded in terms from equations 
\eqref{appendix:eq:sum1}--\eqref{appendix:eq:sum4} and evaluated
as follows:

\begin{equation}
	\begin{split}
		& \sum\limits_{i<s} 2^{-i} \left(
			1 + (-2)^{s+2} - 2^{2i+2} - (-2)^{s+i+3}
		\right) \\
		= & -2^{s+3}  - 2^{1-s} - 2^3(-1)^s + 9.
	\end{split}
\end{equation}

We can now finish the calculation:

\begin{equation}
	\begin{split}
		& \sum\limits_{i<s} 2^{m-i} \xi_i^2 - 2 \xi_s \sum\limits_{i \leq s}  2^{m-i} \xi_i \\
		= & - \frac{2^m}9 \left[
			2^{1-s} (1+(-2)^{s+2} + 2^{2s+2})
			- 2^{s+3}  - 2^{1-s} - 2^3(-1)^s + 9
		\right] \\
		= & -2^m.
	\end{split}
\end{equation}

\subsection{Evaluation of expression in \eqref{z2i:eq:appendixable2}}

Start by rearranging the terms and factoring out the $2^m$ and $2^{-r}$.

\begin{equation}
	\label{appendix:eq:2step1}
	\begin{split}
		& \sum\limits_{i\leq r} 2^{m-i} \xi_i^2
			+ (2^{m-r}-2) \xi_{r+1}^2 + 2\xi_{r+1}((-1)^r 2^m + \xi_{r+1}) \\
			= & \sum\limits_{i\leq r} 2^{m-i} \xi_i^2
				+ 2^{m-r}\xi_{r+1}^2 + 2^{m+1} (-1)^r \xi_{r+1} \\
			= & 2^m \left[
				\sum\limits_{i\leq r} 2^{-i} \xi_i^2
					+ 2^{-r}\xi_{r+1} \left(
						\xi_{r+1} + 2 (-2)^r 
					\right)
			\right].
	\end{split}
\end{equation}

The sum can be evaluated using results \eqref{appendix:eq:xi1} and
\eqref{appendix:eq:sum5}--\eqref{appendix:eq:sum7}:

\begin{equation}
	\begin{split}
		& \sum\limits_{i\leq r} 2^{-i} \xi_i^2 \\
		= & \frac 1 9 \sum\limits_{i\leq r} 2^{-i} \left(
			1 + (-2)^{i+2} + 2^{2i+2}
		\right) \\
		= & \frac 1 9 \left(
			2^{r+3} - 2^{-r} + 2(-1)^r - 9
		\right).
	\end{split}
\end{equation}

The other term was precalculated in \eqref{appendix:eq:xi3}. And we obtain 
the result:

\begin{equation}
	\begin{split}
		& \sum\limits_{i\leq r} 2^{m-i} \xi_i^2
			+ (2^{m-r}-2) \xi_{r+1}^2 + 2\xi_{r+1}((-1)^r 2^m + \xi_{r+1}) \\
		= & \frac {2^m} 9 \left[
			2^{r+3} - 2^{-r} + 2(-1)^r - 9
			+ 2^{-r} \left(
				1 + (-2)^{r+1} + (-2)^{2r+3}
			\right)
		\right] \\
		= & -2^m.
	\end{split}
\end{equation}
